src/normalization/gen_fresh.v
@@ -1,0 +1,94 @@
+From Usuba Require Import usuba_AST collect.
+From Coq Require Import String.
+From Coq Require Import PeanoNat.
+From Coq Require Import MSetFacts.
+Require Import Lia.
+
+Lemma String_append_length:
+    forall (s1 s2 : string),
+        String.length (s1 ++ s2)%string = String.length s1 + String.length s2.
+Proof.
+    intros s1 s2; induction s1; simpl.
+    + reflexivity.
+    + rewrite IHs1; reflexivity.
+Qed.
+
+Lemma leb_add_1_l:
+    forall n, n + 1 <=? n  = false.
+Proof.
+    induction n; simpl; auto.
+Qed.
+
+Fixpoint fill (name : string) (size : nat) : string :=
+    match size with
+    | 0 => name ++ "'"
+    | S size => fill (name ++ "'") size
+    end.
+
+Fixpoint fresh_name_inner (fuel : nat) (size : nat) (name : ident) (s : iset.t) : (ident * nat * iset.t) :=
+    match fuel with
+    | 0 => 
+        let name2 := fill name (size - String.length name) in
+        (name2, max (String.length name + 1) (size + 1), iset.add name2 s)
+    | S fuel' => match iset.mem name s with
+        | true => fresh_name_inner fuel' size (name ++ "'")%string s
+        | false => (name, Nat.max (String.length name) size, iset.add name s)
+        end
+    end.
+
+Definition var_set : Type := nat * iset.t.
+
+Definition var_set_ok (vs : var_set) : Prop :=
+    let (size, vars) := vs in
+        forall name, iset.mem name vars = true -> String.length name <= size.
+
+Definition fresh_name (name : ident) (vs : var_set) : (ident * var_set):=
+    let (size, vars) := vs in
+    let (name_size, vars') := fresh_name_inner 1000 size name vars in
+    let (name', size') := name_size in
+    (name', (size', vars')).
+
+Lemma fill_soundness:
+    forall s name,
+        String.length (fill name s) = String.length name + s + 1.
+Proof.
+    induction s as [|s HRec]; simpl; intro. 
+    + rewrite String_append_length; simpl; lia.
+    + rewrite HRec; rewrite String_append_length; simpl; lia.
+Qed.
+
+Theorem fresh_name_inner_soundness:
+    forall fuel size s name s2 name2 size2,
+        var_set_ok (size, s) ->
+        fresh_name_inner fuel size name s = (name2, size2, s2) ->
+            iset.mem name2 s = false /\ iset.mem name2 s2 = true /\
+            var_set_ok (size2, s2).
+Proof.
+    unfold var_set_ok.
+    induction fuel as [|fuel' HRec]; simpl.
+    all: intros size s name s2 name2 size2 HLength.
+    {
+        intro HEq; inversion HEq.
+        rewrite <- not_true_iff_false.
+        repeat split.
+        + intro Hmem; apply HLength in Hmem; rewrite fill_soundness in Hmem; lia.
+        + rewrite iset.mem_spec; rewrite iset.add_spec; auto.
+        + intros n H; rewrite iset.mem_spec in H; rewrite iset.add_spec in H; destruct H as [H|].
+            - rewrite H; rewrite fill_soundness. lia.
+            - rewrite <- iset.mem_spec in H; apply HLength in H; lia.
+    }
+    case_eq (iset.mem name s); simpl.
+    all: intros Hmem HEq.
+    {
+        apply HRec in HEq; trivial.
+    }
+    {
+        generalize Hmem; clear Hmem.
+        inversion HEq; repeat split; auto.
+        + rewrite iset.mem_spec; rewrite iset.add_spec; auto.
+        + intro; rewrite iset.mem_spec; rewrite iset.add_spec.
+            intro H; destruct H as [H|H].
+            - destruct H; lia.
+            - rewrite <-iset.mem_spec in H; apply HLength in H; lia.
+    }
+Qed.
