src/test_sem.v
@@ -1,18 +1,60 @@
 From mathcomp Require Import all_ssreflect.
-From Usuba Require Import usuba_AST usuba_sem.
+From Usuba Require Import usuba_AST usuba_sem equiv_rel.
 
 Lemma eval_asign:
-    forall arch prog ctxt opt_ctxt' value1 var,
-        find_val ctxt var = Some (ValTuple (lV_cons value1 lV_nil)) ->
-        eval_deq arch prog ctxt
-            (Eqn (VTuple (LVcons (Index (Var var) (Const_e 0)) (LVcons (Index (Var var) (Const_e 0)) LVnil))) (Tuple (ECons (Const 1 None)
+    forall arch prog type_ctxt ctxt opt_ctxt' var typ dir,
+        find_val type_ctxt var = Some typ ->
+        well_typed_ctxt type_ctxt ctxt ->
+        convert_type typ nil = Some (dir, 1::nil) ->
+        eval_deq arch prog type_ctxt ctxt
+            (Eqn (Index (Var var) (Const_e 0) :: (Index (Var var) (Const_e 0)) :: nil) (Tuple (ECons (Const 1 None)
                             (ECons (Const 2 None) Enil)))
                 true) = opt_ctxt'
-        -> (ctxt' <- opt_ctxt'; find_val ctxt' var) = Some (ValTuple (lV_cons (VConst 2) lV_nil)).
+        -> (ctxt' <- opt_ctxt'; find_val ctxt' var) = Some (CoIR dir (2::nil) (Some (1::nil))).
 Proof.
     simpl.
-    move=> _ _ ctxt opt_ctxt val var ->; simpl.
-    rewrite String.eqb_refl.
-    move=> <-; simpl.
-    rewrite String.eqb_refl; reflexivity.
+    unfold bind; unfold bind_aux_list.
+    unfold bind_aux.
+    simpl.
+    move=> _ _ type_ctxt ctxt opt_ctxt var typ dir HEqType well_typed.
+    rewrite HEqType; move=> Convert; rewrite Convert; simpl.
+    case_eq (find_val ctxt var).
+    {
+        move=> c HEq.
+        pose (p := well_typed_ctxt_imp_find_val _ _ _ _ well_typed HEq).
+        destruct p as [typ' [find_typ valoType]].
+        rewrite find_typ in HEqType; inversion HEqType as [HEq'].
+        destruct HEq'; clear HEqType.
+        destruct c as [|d [|hd tl] form]; simpl.
+        {
+            rewrite String.eqb_refl; simpl.
+            move=> <-; simpl.
+            rewrite String.eqb_refl; reflexivity.
+        }
+        {
+            exfalso.
+            apply (val_of_type_len _ _ _ dir _ [:: 1]) in valoType; trivial.
+            simpl in valoType.
+            unfold muln, muln_rec in valoType.
+            rewrite PeanoNat.Nat.mul_1_l in valoType; discriminate.
+        }
+        destruct tl; simpl.
+        {
+            rewrite String.eqb_refl; simpl.
+            move=> <-; simpl.
+            rewrite String.eqb_refl; reflexivity.
+        }
+        {
+            exfalso.
+            apply (val_of_type_len _ _ _ dir _ [:: 1]) in valoType; trivial.
+            simpl in valoType.
+            unfold muln, muln_rec in valoType.
+            rewrite PeanoNat.Nat.mul_1_l in valoType; discriminate.
+        }
+    }
+    {
+        move=> _; simpl; rewrite String.eqb_refl; simpl.
+        move=> <-; simpl.
+        rewrite String.eqb_refl; reflexivity.
+    }
 Qed.
