src/utils.v
@@ -1,0 +1,24 @@
+From mathcomp Require Import all_ssreflect.
+
+Ltac impl_tac :=
+    lazymatch goal with
+    | |- (?A -> ?B) -> ?C =>
+        let H := fresh "H" in
+        let H2 := fresh "H" in
+        let H3 := fresh "H" in
+        assert A as H; [> idtac | (move=> H2; pose (H3 := H2 H); move: H3; clear H2 H)]
+    end.
+
+Ltac eq_match :=
+    lazymatch goal with
+    | |- match ?A with Some _ => _ | None => _ end = match ?B with Some _ => _ | None => _  end =>
+        let H := fresh "H" in
+        assert (A = B) as H; [> idtac | rewrite H; reflexivity]
+    end.
+
+Ltac small_eq_match :=
+    lazymatch goal with
+    | |- match ?A with Some _ => _ | None => _ end = match ?B with Some _ => _ | None => _  end =>
+        let H := fresh "H" in
+        assert (A = B) as H; [> idtac | rewrite H; destruct B]
+    end.
